Cslib.lean
@@ -46,9 +46,11 @@ public import Cslib.Computability.Languages.OmegaLanguage
 public import Cslib.Computability.Languages.OmegaRegularLanguage
 public import Cslib.Computability.Languages.RegularLanguage
 public import Cslib.Computability.Languages.SafetyLiveness
+public import Cslib.Computability.Machines.Turing.MultiTape.Combinators.Concat
 public import Cslib.Computability.Machines.Turing.MultiTape.Deterministic
 public import Cslib.Computability.Machines.Turing.MultiTape.NormalForms.RewindInput
 public import Cslib.Computability.Machines.Turing.MultiTape.Plumbing.Basic
+public import Cslib.Computability.Machines.Turing.MultiTape.Plumbing.Concat
 public import Cslib.Computability.Machines.Turing.MultiTape.Plumbing.ExtendTapes
 public import Cslib.Computability.Machines.Turing.MultiTape.Plumbing.InputFromWorkTape
 public import Cslib.Computability.Machines.Turing.MultiTape.Plumbing.InputFromWorkTape.Defs
